implicit-monads/AdditiveMonads.v
@@ -1,0 +1,71 @@
+(** Formalization of monads with a commutative sum operation to combine them.
+    See StrongMonads.v for a better version. *)
+Require Import String.
+
+Set Implicit Arguments.
+
+Class Monad : Type := {
+  I : Type;
+  O : Type;
+  E : Type;
+  M : Type -> Type :=
+    fun A => I -> (A + E) * O;
+  ret : forall A, A -> M A;
+  bind : forall A B, M A -> (A -> M B) -> M B}.
+
+Definition monadic_sum {m1 m2 : Monad} : Monad := {|
+  I := @I m1 * @I m2;
+  O := @O m1 * @O m2;
+  E := @E m1 + @E m2;
+  ret := fun _ x i =>
+    let (i1, i2) := i in
+    match (ret x i1, ret x i2) with
+    | ((inl _, o1), (inl _, o2)) => (inl x, (o1, o2))
+    | ((inl _, o1), (inr e2, o2)) => (inr (inr e2), (o1, o2))
+    | ((inr e1, o1), (_, o2)) => (inr (inl e1), (o1, o2))
+    end;
+  bind := fun _ _ x f i =>
+     match x i with
+     | (inl x', (o1, o2)) =>
+      let x1 := fun i1 => 
+      end
+     | (inr e, (o1, o2) => (inr e, (o1, o2))
+     end |}.
+
+Infix "·" := monadic_sum (at level 50, left associativity).
+
+Instance Id : Monad := {
+  I := unit;
+  O := unit;
+  E := Empty_set;
+  ret := fun _ x _ => (inl x, tt)}.
+
+Instance Option : Monad := {
+  I := unit;
+  O := unit;
+  E := unit;
+  ret := fun _ x _ => (inl x, tt)}.
+
+Instance Error (E : Type) : Monad := {
+  I := unit;
+  O := unit;
+  E := E;
+  ret := fun _ x _ => (inl x, tt)}.
+
+Instance Print : Monad := {
+  I := unit;
+  O := list string;
+  E := Empty_set;
+  ret := fun _ x _ => (inl x, nil)}.
+
+Instance State (S : Type) : Monad := {
+  I := S;
+  O := S;
+  E := Empty_set;
+  ret := fun _ x s => (inl x, s)}.
+
+Instance Loop : Monad := {
+  I := nat;
+  O := unit;
+  E := unit;
+  ret := fun _ x _ => (inl x, tt)}.
