implicit-monads/OpenMonads.v
@@ -1,0 +1,40 @@
+(** Monads with an open structure to give more freedom to the run operations *)
+
+Set Implicit Arguments.
+
+Class Monad : Type := {
+  I : Type;
+  E : Type;
+  O : Type;
+  O_of_I : I -> O}.
+
+Module M.
+  Inductive t {m : Monad} (A : Type) : Type :=
+  | new : (I -> (A + E + t A) * O) -> t A.
+End M.
+
+Definition ret {m : Monad} A (x : A) : M.t A :=
+  M.new (fun i => (inl (inl x), O_of_I i)).
+
+Fixpoint bind {m : Monad} A B (x : M.t A) (f : A -> M.t B) : M.t B :=
+  M.new (fun i =>
+    match x with
+    | M.new x =>
+      match x i with
+      | (inl xe, o) =>
+        match xe with
+        | inl x => (inr (f x), o)
+        | inr e => (inl (inr e), o)
+        end
+      | (inr x, o) => (inr (bind x f), o)
+      end
+    end).
+
+Fixpoint run {m : Monad} A (x : M.t A) (I_of_O : O -> I) (i : I) : (A + E) * O :=
+  match x with
+  | M.new x =>
+    match x i with
+    | (inl xe, o) => (xe, o)
+    | (inr x, o) => run x I_of_O (I_of_O o)
+    end
+  end.
